save

Hnr.thy
@@ -1,8 +1,8 @@
 theory Hnr 
-  imports Array_Safe Diff_Arr
+  imports Array_Safe Diff_Arr_Safe
 begin
 
-definition hnr where "hnr \<Gamma> c \<Gamma>' R a = <\<Gamma>> c <\<lambda>r. \<Gamma>' * R a r>\<^sub>t"
+definition hnr where "hnr \<Gamma> c \<Gamma>' a = <\<Gamma>> c <\<lambda>r. \<Gamma>' a r>\<^sub>t"
 
 lemmas hnrD = hnr_def[THEN iffD1]
 lemmas hnrI = hnr_def[THEN iffD2]
@@ -13,11 +13,12 @@ abbreviation id_assn where "id_assn a c \<equiv> \<up>(id_rel a c)"
 
 abbreviation array_assn where "array_assn xs xsi \<equiv> xsi \<mapsto>\<^sub>a xs"
 
-named_theorems hnr_rule
 named_theorems hnr_rule_raw
+
+named_theorems hnr_rule_arr
 named_theorems hnr_rule_diff_arr
 
-lemma hnr_return: "hnr \<Gamma> (return x) \<Gamma> id_assn x"
+lemma hnr_return: "hnr \<Gamma> (return x) (\<lambda> x xi. \<Gamma> * id_assn x xi) x"
   unfolding hnr_def id_rel_def
   by sep_auto
 
@@ -58,11 +59,11 @@ method keep_drop =
 
 lemma hnr_let[hnr_rule_raw]:
   assumes 
-    "hnr \<Gamma> vi \<Gamma>\<^sub>1 R\<^sub>1 v" 
-    "\<And>xi x. hnr (\<Gamma>\<^sub>1 * R\<^sub>1 x xi) (fi xi) (\<Gamma>' x xi) R (f x)"
-    "\<And>xi x. keep_drop (\<Gamma>' x xi) \<Gamma>'' (R\<^sub>1' x xi)"
+    "hnr \<Gamma> vi \<Gamma>\<^sub>1 v" 
+    "\<And>xi x. hnr (\<Gamma>\<^sub>1 x xi) (fi xi) (\<Gamma>' x xi) (f x)"
+    "\<And>xi x ri r. keep_drop (\<Gamma>' x xi r ri) (\<Gamma>'' r ri) (\<Gamma>\<^sub>1' x xi r ri)"
   shows 
-    "hnr \<Gamma> (do { x \<leftarrow> vi; fi x }) \<Gamma>'' R (let x = v in f x)"
+    "hnr \<Gamma> (do { x \<leftarrow> vi; fi x }) \<Gamma>'' (let x = v in f x)"
   supply[sep_heap_rules] = assms(1, 2)[THEN hnrD]
   apply(rule hnrI)
   apply sep_auto
@@ -71,14 +72,27 @@ lemma hnr_let[hnr_rule_raw]:
 
 lemma hnr_if: 
   assumes
-    "hnr \<Gamma> ai \<Gamma>\<^sub>a R\<^sub>a a"
-    "hnr \<Gamma> bi \<Gamma>\<^sub>b R\<^sub>b b"
+    "hnr \<Gamma> ai \<Gamma>\<^sub>a a"
+    "hnr \<Gamma> bi \<Gamma>\<^sub>b b"
   shows 
     "hnr 
       \<Gamma> 
       (if c then ai else bi) 
-      (\<Gamma>\<^sub>a \<or>\<^sub>A \<Gamma>\<^sub>b) 
-      (\<lambda>a r. R\<^sub>a a r * \<up> c \<or>\<^sub>A R\<^sub>b a r * \<up>(\<not>c)) 
+      (\<lambda>a r. \<Gamma>\<^sub>a a r \<or>\<^sub>A \<Gamma>\<^sub>b a r) 
+      (if c then a else b)" 
+  supply[sep_heap_rules] = assms[THEN hnrD]
+  apply(rule hnrI)
+  by(sep_auto simp: ent_star_mono)
+
+lemma hnr_if': 
+  assumes
+    "hnr \<Gamma> ai \<Gamma>\<^sub>a a"
+    "hnr \<Gamma> bi \<Gamma>\<^sub>b b"
+  shows 
+    "hnr 
+      \<Gamma> 
+      (if c then ai else bi) 
+      (\<lambda>a r. \<Gamma>\<^sub>a a r * \<up> c \<or>\<^sub>A \<Gamma>\<^sub>b a r * \<up>(\<not>c)) 
       (if c then a else b)" 
   supply[sep_heap_rules] = assms[THEN hnrD]
   apply(rule hnrI)
@@ -103,49 +117,52 @@ shows
   sorry *)
 
 
-lemma hnr_array_nth [hnr_rule]: "
+lemma hnr_array_nth [hnr_rule_arr]: "
     hnr
      (xsi \<mapsto>\<^sub>a xs * id_assn i ii)
      (array_nth_safe xsi ii) 
-     (xsi \<mapsto>\<^sub>a xs * id_assn i ii) 
-     id_assn 
+     (\<lambda> r ri. xsi \<mapsto>\<^sub>a xs * id_assn r ri) 
      (xs ! i)"
   unfolding id_rel_def
   apply(rule hnrI)
   by sep_auto
 
-lemma hnr_array_update [hnr_rule]: "
+lemma hnr_array_update [hnr_rule_arr]: "
     hnr 
       (xsi \<mapsto>\<^sub>a xs * id_assn i ii * id_assn v vi) 
       (array_update_safe ii vi xsi) 
-      (id_assn i ii * id_assn v vi) 
-      array_assn 
+      array_assn
       (xs [i:= v])"
   unfolding id_rel_def
   apply(rule hnrI)
   by sep_auto
 
-lemma hnr_pass: "hnr (A x xi) (return xi) emp A x"
+lemma hnr_pass: "hnr (A x xi) (return xi) A x"
   unfolding id_rel_def
   apply(rule hnrI)
   by sep_auto
 
-lemma hnr_copy: "hnr (id_assn x xi) (return xi) emp id_assn x"
+lemma hnr_copy: "hnr (id_assn x xi) (return xi) id_assn x"
   unfolding id_rel_def
   apply(rule hnrI)
   by sep_auto
 
 lemma hnr_copy_diff_arr [hnr_rule_diff_arr]:
-  "hnr (master_assn t * \<up>(t \<turnstile> x \<sim> xi)) (return xi) (master_assn t) (\<lambda>x xi. \<up>(t \<turnstile> x \<sim> xi)) x"
+  "hnr (master_assn t * \<up>(t \<turnstile> x \<sim> xi)) (return xi) (\<lambda>x xi. master_assn t * \<up>(t \<turnstile> x \<sim> xi)) x"
+  apply(rule hnrI)
+  by sep_auto
+
+lemma hnr_copy_arr [hnr_rule_arr]:
+  "hnr (array_assn x xi) (return xi) array_assn x"
   apply(rule hnrI)
   by sep_auto
 
 lemma hnr_frame:
   assumes
     "\<Gamma>\<^sub>P \<Longrightarrow>\<^sub>A \<Gamma> * F"
-    "hnr \<Gamma> fi \<Gamma>' R f"
+    "hnr \<Gamma> fi \<Gamma>' f"
   shows
-    "hnr \<Gamma>\<^sub>P fi (\<Gamma>' * F) R f"
+    "hnr \<Gamma>\<^sub>P fi (\<lambda> r ri. \<Gamma>' r ri * F) f"
   apply(rule hnrI)
   by (smt (verit) assms(1) assms(2) assn_aci(10) fi_rule hnrD hoare_triple_def)
 
@@ -153,8 +170,7 @@ lemma hnr_lookup[hnr_rule_diff_arr]: "
   hnr
     (master_assn t * id_assn i ii * \<up>(t \<turnstile> xs \<sim> xsi))
     (diff_arr_lookup_safe xsi ii)
-    (master_assn t)
-    id_assn
+    (\<lambda>r ri. master_assn t * id_assn r ri)
     (xs ! i)"
   unfolding id_rel_def
   apply(rule hnrI)
@@ -164,31 +180,25 @@ lemma hnr_realize: "
   hnr
     (master_assn t * \<up>(t \<turnstile> xs \<sim> xsi))
     (Diff_Arr.realize xsi)
-    (master_assn t * \<up>(t \<turnstile> xs \<sim> xsi))
-    array_assn
+    (\<lambda> r ri. master_assn t  * array_assn r ri)
     xs"
   unfolding id_rel_def
   apply(rule hnrI)
   using realize[of t xs xsi]
   by(sep_auto simp: cons_post_rule ent_refl_true)
 
-lemma ht_combine_post: "<P> c <Q> \<Longrightarrow> <P> c <Q'> \<Longrightarrow> <P> c <\<lambda>r. Q r \<and>\<^sub>A Q' r>"
-  unfolding hoare_triple_def
-  by(auto simp: Let_def mod_and_dist)
-
 lemma hnr_update[hnr_rule_diff_arr]: "
   hnr
     (master_assn t * \<up>(t \<turnstile> xs \<sim> xsi) * id_assn i ii * id_assn v vi)
     (diff_arr_update_safe xsi ii vi)
-    (id_assn i ii * id_assn v vi)
-    (\<lambda>xs xsi. \<exists>\<^sub>At'. master_assn t' * \<up>((\<forall>xs' xsi'. t \<turnstile> xs' \<sim>  xsi' \<longrightarrow> t' \<turnstile> xs' \<sim>  xsi') \<and> t' \<turnstile> xs \<sim> xsi))
+    (\<lambda>xs xsi. \<exists>\<^sub>At'. master_assn t' * 
+              \<up>((\<forall>xs' xsi'. t \<turnstile> xs' \<sim>  xsi' \<longrightarrow> t' \<turnstile> xs' \<sim>  xsi') \<and> t' \<turnstile> xs \<sim> xsi))
     (xs [i:= v])"
   unfolding id_rel_def
   apply(rule hnrI)
   apply(sep_auto)
   apply(rule cons_post_rule)
-   apply(rule fi_rule[OF update_safe])
-  apply solve_entails
-  by sep_auto
+  apply(rule fi_rule[OF update_safe])
+  by sep_auto+
 
 end
