Array_Safe.thy
@@ -1,5 +1,5 @@
 theory Array_Safe
-  imports  Diff_Arr
+  imports Base
 begin
 
 (* TODO: Use locale? *)
@@ -23,29 +23,9 @@ definition array_update_safe where
     else return arr
   }"
 
-definition diff_arr_lookup_safe where
-  "diff_arr_lookup_safe arr i = do {
-    len \<leftarrow>  Diff_Arr.length arr;
-    if i < len
-    then  Diff_Arr.lookup arr i
-    else do { 
-      arr \<leftarrow>  Diff_Arr.realize arr;
-      xs \<leftarrow> Array.freeze arr;
-      return (xs ! i)
-    }
-  }"
-
-definition diff_arr_update_safe  where
-  "diff_arr_update_safe arr i v = do {
-    len \<leftarrow>  Diff_Arr.length arr;
-    if i < len
-    then Diff_Arr.update arr i v 
-    else return arr
-  }"
-
 lemma nth_undefined: "i \<ge> length xs \<Longrightarrow> xs ! i = undefined(i - length xs)"
-  apply(induction xs arbitrary: i)
   unfolding List.nth_def
+  apply(induction xs arbitrary: i)
   by(auto split: nat.splits)
 
 lemma array_nth_safe [sep_heap_rules]: "
@@ -53,41 +33,11 @@ lemma array_nth_safe [sep_heap_rules]: "
     array_nth_safe arr i
    <\<lambda>res. \<up>(res = xs ! i) * arr \<mapsto>\<^sub>a xs>"
   unfolding array_nth_safe_def
-  by(sep_auto simp: nth_undefined)
+  by sep_auto
 
 lemma array_update_safe [sep_heap_rules]:
   "<arr \<mapsto>\<^sub>a xs> array_update_safe i v arr <\<lambda>res. \<up>(res = arr) * arr \<mapsto>\<^sub>a xs[i := v]>"
   unfolding array_update_safe_def
   by sep_auto
-
-lemma update_safe[sep_heap_rules]: "
-  <master_assn t * \<up>(t \<turnstile> xs \<sim> diff_arr)> 
-     diff_arr_update_safe diff_arr i v
-  <\<lambda>diff_arr. \<exists>\<^sub>At'. master_assn t' * 
-    \<up>((\<forall>xs' diff_arr'. t \<turnstile> xs' \<sim> diff_arr' \<longrightarrow> t' \<turnstile> xs' \<sim> diff_arr') 
-      \<and> (t' \<turnstile> xs[i := v] \<sim> diff_arr))>\<^sub>t
-"
-  unfolding diff_arr_update_safe_def
-  apply sep_auto
-   apply(rule fi_rule[OF length])
-   apply sep_auto
-  apply sep_auto
-   apply(rule cons_post_rule)
-    apply(rule fi_rule[OF update])
-  by sep_auto+
-
-lemma lookup_safe [sep_heap_rules]: "
-  <master_assn t * \<up>(t \<turnstile> xs \<sim> a)> 
-     diff_arr_lookup_safe a i 
-  <\<lambda>r. master_assn t * \<up>(r = xs!i)>\<^sub>t"
-  unfolding diff_arr_lookup_safe_def
-  apply sep_auto
-   apply(rule fi_rule[OF length])
-   apply sep_auto+
-  apply(rule cons_post_rule)
-    apply(rule fi_rule[OF lookup])
-    apply sep_auto+
-   apply(rule fi_rule[OF realize])
-  by sep_auto+
 
 end
